Excellent example ðŸ‘
This code is **exactly about how `detach()` breaks the computation graph** and how gradients flow mathematically.

Letâ€™s go step-by-step and do the math.

---

# ðŸ§© The Code

```python
x.grad.zero_()

y = x * x
u = y.detach()
z = u * x
z.sum().backward()

x.grad == u
```

Assume:

```python
x = [x0, x1, x2, x3] = [0, 1, 2, 3]
```

---

# ðŸ§  Step 1 â€” Reset gradient

```python
x.grad.zero_()
```

Now:

[
x.grad = [0,0,0,0]
]

Nothing else changes.

---

---

# ðŸŸ¢ Step 2 â€” Compute y = x * x

```python
y = x * x
```

Mathematically:

[
y_i = x_i^2
]

So:

[
y = [0^2, 1^2, 2^2, 3^2] = [0,1,4,9]
]

âš ï¸ At this point, `y` is connected to `x` in the computation graph.

---

---

# ðŸ”´ Step 3 â€” Detach y

```python
u = y.detach()
```

This is the MOST IMPORTANT LINE.

`detach()` means:

> ðŸš« Stop gradient tracking here.
> `u` is treated as a constant.

Mathematically:

[
u = [0,1,4,9] \quad \text{(constant, no gradient)}
]

Even though numerically equal to `y`, autograd will not compute gradients through `u`.

Graph becomes:

```
x â”€â”€â–º y    (graph stops here)
u = constant
```

---

---

# ðŸŸ¢ Step 4 â€” Compute z = u * x

```python
z = u * x
```

Elementwise multiplication:

[
z_i = u_i \cdot x_i
]

So:

[
z = [0Â·0, 1Â·1, 4Â·2, 9Â·3] = [0, 1, 8, 27]
]

---

---

# ðŸŸ¢ Step 5 â€” Sum

```python
z.sum()
```

[
s = \sum_i z_i = \sum_i u_i x_i
]

This is:

[
s = u_0 x_0 + u_1 x_1 + u_2 x_2 + u_3 x_3
]

---

---

# ðŸ”™ Step 6 â€” Backward (Derivative)

We compute:

[
\frac{âˆ‚s}{âˆ‚x_i}
]

Since:

[
s = \sum_i u_i x_i
]

and **u is constant**, derivative is:

[
\frac{âˆ‚s}{âˆ‚x_i} = u_i
]

So gradient is:

[
x.grad = [u_0, u_1, u_2, u_3]
]

Which equals:

[
x.grad = u
]

---

---

# âœ… That is why:

```python
x.grad == u
```

returns:

```
True
```

---

---

# ðŸŽ¯ Final Mathematical Flow Summary

Let:

[
x = [x_i]
]

1. **Square**
   [
   y_i = x_i^2
   ]

2. **Detach**
   [
   u_i = y_i \quad \text{(treated as constant)}
   ]

3. **Multiply**
   [
   z_i = u_i x_i
   ]

4. **Sum**
   [
   s = \sum_i u_i x_i
   ]

5. **Gradient**
   [
   \frac{âˆ‚s}{âˆ‚x_i} = u_i
   ]

---

---

# âš ï¸ Very Important Insight

If you **did NOT detach**, then:

[
z = (x^2) x = x^3
]

[
s = \sum_i x_i^3
]

Derivative would be:

[
\frac{âˆ‚s}{âˆ‚x_i} = 3x_i^2
]

But because of `detach()`, PyTorch blocks that path.

---

---

# ðŸ§  Intuition

> ðŸ”¥ `detach()` freezes a tensor and treats it like a constant in math.

---

---

# âœ… One-line Answer

Because `u` is detached, gradient flows only through `x` in:

[
s = \sum u_i x_i
]

So gradient equals:

[
x.grad = u
]

---

If you want, I can also show:
âœ… What happens WITHOUT detach
âœ… Graph diagrams
âœ… Why detach is used in GANs / RL
âœ… Memory optimization tricks
